Rename AutomataOI2 to Automaton.OI2

AutomataTheory/AutomataOI2.lean
@@ -25,21 +25,21 @@ open Classical
 
 variable {A : Type*} (M : Fin 2 → Automaton A) (acc : (i : Fin 2) → Set ((M i).State))
 
-def AutomataOI2_HistInit : Set (Fin 2) := {0}
+def Automaton.OI2_HistInit : Set (Fin 2) := {0}
 
-def AutomataOI2_HistNext : (Automaton.Prod M).State × Fin 2 → A → Set (Fin 2) :=
+def Automaton.OI2_HistNext : (Automaton.Prod M).State × Fin 2 → A → Set (Fin 2) :=
   fun s _ ↦
     if s.1 0 ∈ acc 0 ∧ s.2 = 0 then {1} else
     if s.1 1 ∈ acc 1 ∧ s.2 = 1 then {0} else {s.2}
 
-def AutomataOI2 : Automaton A :=
-  (Automaton.Prod M).addHist AutomataOI2_HistInit (AutomataOI2_HistNext M acc)
+def Automaton.OI2 : Automaton A :=
+  (Automaton.Prod M).addHist Automaton.OI2_HistInit (Automaton.OI2_HistNext M acc)
 
-def AutomataOI2_Acc : Set (AutomataOI2 M acc).State :=
+def Automaton.OI2_Acc : Set (Automaton.OI2 M acc).State :=
   { s | s.1 0 ∈ acc 0 ∧ s.2 = 0 } ∪ { s | s.1 1 ∈ acc 1 ∧ s.2 = 1 }
 
-private lemma automata_oi2_lemma1 {as : ℕ → A} {ss : ℕ → (AutomataOI2 M acc).State}
-    (h_run : InfRun (AutomataOI2 M acc) as ss) :
+private lemma automata_oi2_lemma1 {as : ℕ → A} {ss : ℕ → (Automaton.OI2 M acc).State}
+    (h_run : InfRun (Automaton.OI2 M acc) as ss) :
       (∃ᶠ k in atTop, ss k ∈ { s | s.1 0 ∈ acc 0 ∧ s.2 = 0 }) ↔
       (∃ᶠ k in atTop, ss k ∈ { s | s.1 1 ∈ acc 1 ∧ s.2 = 1 }) := by
   constructor <;> intro h_inf
@@ -49,7 +49,7 @@ private lemma automata_oi2_lemma1 {as : ℕ → A} {ss : ℕ → (AutomataOI2 M 
       apply leads_to_step ; simp [Step]
       intro k h_acc h_hist
       have h_step := (h_run.2 k).2
-      simp [AutomataOI2_HistNext, h_acc, h_hist] at h_step
+      simp [Automaton.OI2_HistNext, h_acc, h_hist] at h_step
       assumption
     have h_lt2 : LeadsTo ss {s | s.2 = 1} {s | s.1 1 ∈ acc 1 ∧ s.2 = 1} := by
       apply leads_to_until_frequently_1
@@ -58,7 +58,7 @@ private lemma automata_oi2_lemma1 {as : ℕ → A} {ss : ℕ → (AutomataOI2 M 
         rw [imp_not_comm] at h_acc
         have h_acc := h_acc h_hist
         have h_step := (h_run.2 k).2
-        simp [AutomataOI2_HistNext, h_acc, h_hist] at h_step
+        simp [Automaton.OI2_HistNext, h_acc, h_hist] at h_step
         assumption
       · let p k := ss k ∈ {s | s.1 0 ∈ acc 0 ∧ s.2 = 0}
         let q k := ss k ∉ {s | s.2 = 1}
@@ -73,7 +73,7 @@ private lemma automata_oi2_lemma1 {as : ℕ → A} {ss : ℕ → (AutomataOI2 M 
       apply leads_to_step ; simp [Step]
       intro k h_acc h_hist
       have h_step := (h_run.2 k).2
-      simp [AutomataOI2_HistNext, h_acc, h_hist] at h_step
+      simp [Automaton.OI2_HistNext, h_acc, h_hist] at h_step
       assumption
     have h_lt2 : LeadsTo ss {s | s.2 = 0} {s | s.1 0 ∈ acc 0 ∧ s.2 = 0} := by
       apply leads_to_until_frequently_1
@@ -82,7 +82,7 @@ private lemma automata_oi2_lemma1 {as : ℕ → A} {ss : ℕ → (AutomataOI2 M 
         rw [imp_not_comm] at h_acc
         have h_acc := h_acc h_hist
         have h_step := (h_run.2 k).2
-        simp [AutomataOI2_HistNext, h_acc, h_hist] at h_step
+        simp [Automaton.OI2_HistNext, h_acc, h_hist] at h_step
         assumption
       · let p k := ss k ∈ {s | s.1 1 ∈ acc 1 ∧ s.2 = 1}
         let q k := ss k ∉ {s | s.2 = 0}
@@ -92,26 +92,26 @@ private lemma automata_oi2_lemma1 {as : ℕ → A} {ss : ℕ → (AutomataOI2 M 
         exact Frequently.mono h_inf h_imp
     exact leads_to_trans h_lt1 h_lt2
 
-private lemma automata_oi2_lemma2 {as : ℕ → A} {ss : ℕ → (AutomataOI2 M acc).State}
-    (h_run : InfRun (AutomataOI2 M acc) as ss)
+private lemma automata_oi2_lemma2 {as : ℕ → A} {ss : ℕ → (Automaton.OI2 M acc).State}
+    (h_run : InfRun (Automaton.OI2 M acc) as ss)
     (h_inf0 : ∃ᶠ k in atTop, ss k ∈ { s | s.1 0 ∈ acc 0 })
     (h_inf1 : ∃ᶠ k in atTop, ss k ∈ { s | s.1 1 ∈ acc 1 }) :
       ∃ᶠ k in atTop, ss k ∈ { s | s.1 0 ∈ acc 0 ∧ s.2 = 0 } ∪ { s | s.1 1 ∈ acc 1 ∧ s.2 = 1 } := by
   have h_true : ∃ᶠ k in atTop, ss k ∈ univ := by simp [atTop_neBot]
   apply frequently_leads_to_frequently h_true
   apply leads_to_cases (p := univ) (q := {s | s.2 = 0}) <;> simp [univ_inter]
-  · have h_inter : {s : (AutomataOI2 M acc).State | s.1 0 ∈ acc 0 ∧ s.2 = 0} = {s | s.2 = 0} ∩ {s | s.1 0 ∈ acc 0} := by
+  · have h_inter : {s : (Automaton.OI2 M acc).State | s.1 0 ∈ acc 0 ∧ s.2 = 0} = {s | s.2 = 0} ∩ {s | s.1 0 ∈ acc 0} := by
       ext s ; simp ; tauto
     rw [h_inter]
     apply leads_to_until_frequently_2 (h2 := h_inf0)
     simp [Step]
     intro k h_hist h_acc
     have h_step := (h_run.2 k).2
-    simp [AutomataOI2_HistNext, h_acc, h_hist] at h_step
+    simp [Automaton.OI2_HistNext, h_acc, h_hist] at h_step
     assumption
-  · have h_inter : {s : (AutomataOI2 M acc).State | s.1 1 ∈ acc 1 ∧ s.2 = 1} = {s | s.2 = 1} ∩ {s | s.1 1 ∈ acc 1} := by
+  · have h_inter : {s : (Automaton.OI2 M acc).State | s.1 1 ∈ acc 1 ∧ s.2 = 1} = {s | s.2 = 1} ∩ {s | s.1 1 ∈ acc 1} := by
       ext s ; simp ; tauto
-    have h_compl : {s : (AutomataOI2 M acc).State | s.2 = 0}ᶜ = {s | s.2 = 1} := by
+    have h_compl : {s : (Automaton.OI2 M acc).State | s.2 = 0}ᶜ = {s | s.2 = 1} := by
       ext s ; simp
       constructor
       · exact Fin.eq_one_of_ne_zero s.2
@@ -121,15 +121,15 @@ private lemma automata_oi2_lemma2 {as : ℕ → A} {ss : ℕ → (AutomataOI2 M 
     simp [Step]
     intro k h_hist h_acc
     have h_step := (h_run.2 k).2
-    simp [AutomataOI2_HistNext, h_acc, h_hist] at h_step
+    simp [Automaton.OI2_HistNext, h_acc, h_hist] at h_step
     assumption
 
 theorem accepted_omega_lang_inter2 :
-    AcceptedOmegaLang (AutomataOI2 M acc) (AutomataOI2_Acc M acc) = ⋂ i : Fin 2, AcceptedOmegaLang (M i) (acc i) := by
+    AcceptedOmegaLang (Automaton.OI2 M acc) (Automaton.OI2_Acc M acc) = ⋂ i : Fin 2, AcceptedOmegaLang (M i) (acc i) := by
   ext as ; simp [AcceptedOmegaLang, BuchiAccept]
   constructor
   · rintro ⟨ss, h_run, h_inf⟩ i
-    have h_run1 := automata_hist_inf_run_proj (Automaton.Prod M) AutomataOI2_HistInit (AutomataOI2_HistNext M acc) h_run
+    have h_run1 := automata_hist_inf_run_proj (Automaton.Prod M) Automaton.OI2_HistInit (Automaton.OI2_HistNext M acc) h_run
     have h_run' := automata_prod_inf_run.mp h_run1 i
 --    have h_run' := (automata_prod_inf_run M as (Prod.fst ∘ ss)).mp h_run1 i
     use (fun k ↦ (Prod.fst ∘ ss) k i) ; constructor
@@ -157,12 +157,12 @@ theorem accepted_omega_lang_inter2 :
     let ss' := fun k i ↦ ss i k
     have h_ss' : ∀ i, InfRun (M i) as (fun k ↦ ss' k i) := by intro i ; exact (h_ss i).1
     have h_run' := automata_prod_inf_run.mpr h_ss'
-    have h_hist_init : AutomataOI2_HistInit.Nonempty := by simp [AutomataOI2_HistInit]
-    have h_hist_next : ∀ s a, (AutomataOI2_HistNext M acc s a).Nonempty := by
-      intro s a ; simp only [AutomataOI2_HistNext]
+    have h_hist_init : Automaton.OI2_HistInit.Nonempty := by simp [Automaton.OI2_HistInit]
+    have h_hist_next : ∀ s a, (Automaton.OI2_HistNext M acc s a).Nonempty := by
+      intro s a ; simp only [Automaton.OI2_HistNext]
       rcases Classical.em (s.1 0 ∈ acc 0 ∧ s.2 = 0) with cond1 | cond1 <;> simp [cond1]
       rcases Classical.em (s.1 1 ∈ acc 1 ∧ s.2 = 1) with cond2 | cond2 <;> simp [cond2]
-    have h_runh := automata_hist_inf_run_exists (Automaton.Prod M) AutomataOI2_HistInit (AutomataOI2_HistNext M acc)
+    have h_runh := automata_hist_inf_run_exists (Automaton.Prod M) Automaton.OI2_HistInit (Automaton.OI2_HistNext M acc)
       h_hist_init h_hist_next h_run'
     obtain ⟨hs, h_run⟩ := h_runh
     use (fun k ↦ (ss' k, hs k))
